src/OperationalSemantics.v
@@ -1,0 +1,661 @@
+Require Import Prog.
+Require Import Word AsyncDisk.
+Require Import Mem Pred PredCrash.
+
+Require Import FunctionalExtensionality.
+Require Import List.
+Require Import Arith.PeanoNat.
+Require Import RelationClasses.
+
+Set Implicit Arguments.
+
+Arguments possible_sync {AT AEQ} _ _.
+Hint Resolve possible_sync_refl.
+Hint Resolve possible_sync_trans.
+
+Ltac inv_opt :=
+  repeat match goal with
+         | [ H: Some _ = Some _ |- _ ] =>
+           inversion H; subst; clear H
+         | [ H: Some _ = None |- _ ] =>
+           solve [ inversion H ]
+         | [ H: None = Some _ |- _ ] =>
+           solve [ inversion H ]
+         end.
+
+Ltac sigT_eq :=
+  match goal with
+  | [ H: @eq (sigT _) _ _ |- _ ] =>
+    apply ProofIrrelevance.ProofIrrelevanceTheory.EqdepTheory.inj_pair2 in H;
+    subst
+  end.
+
+Section StepPreSync.
+Arguments possible_sync {AT AEQ} _ _.
+  Hint Constructors step.
+  Hint Resolve ListUtils.incl_cons2.
+
+  Lemma possible_sync_respects_upd : forall A AEQ (m m': @mem A AEQ _)
+                                       a v l l',
+      possible_sync m m' ->
+      incl l' l ->
+      possible_sync (upd m a (v, l)) (upd m' a (v,l')).
+  Proof.
+    unfold possible_sync; intros.
+    destruct (AEQ a a0); subst; autorewrite with upd;
+      intuition eauto.
+    specialize (H a0); intuition auto.
+    right; repeat eexists; eauto.
+    repeat deex.
+    right; repeat eexists; eauto.
+  Qed.
+
+  Hint Resolve incl_refl.
+
+  Lemma possible_sync_respects_sync_mem : forall A AEQ (m m': @mem A AEQ _),
+      possible_sync m m' ->
+      possible_sync (sync_mem m) (sync_mem m').
+  Proof.
+    unfold possible_sync, sync_mem; intros.
+    specialize (H a).
+    destruct (m a) as [ [] | ];
+    destruct (m' a) as [ [] | ];
+      subst; intuition eauto;
+      try congruence;
+      repeat deex;
+      inv_opt;
+      right.
+    do 3 eexists; intuition eauto.
+  Qed.
+
+  Hint Resolve possible_sync_respects_upd.
+  Hint Resolve possible_sync_respects_sync_mem.
+
+  Theorem step_presync : forall T (m m' m'' m''': rawdisk) hm (p: prog T) hm' v,
+      possible_sync (AEQ:=Nat.eq_dec) m m' ->
+      step m' hm p m'' hm' v ->
+      possible_sync (AEQ:=Nat.eq_dec) m'' m''' ->
+      exists (m'2: rawdisk),
+        step m hm p m'2 hm' v /\
+        possible_sync (AEQ:=Nat.eq_dec) m'2 m'''.
+  Proof.
+    intros.
+    inversion H0; subst; repeat sigT_eq; eauto.
+    - exists m; intuition eauto.
+      specialize (H a); intuition auto; repeat deex; try congruence.
+      assert (v = v0) by congruence; subst.
+      eauto.
+    - pose proof (H a); intuition auto; try congruence.
+      repeat deex.
+      assert (v = v1) by congruence.
+      assert (x = l') by congruence.
+      subst.
+      exists (upd m a (v0, v1::l)).
+      intuition eauto.
+    - pose proof (H a); intuition auto; try congruence.
+      repeat deex.
+      eauto.
+      exists (upd m a vs').
+      destruct vs'.
+      intuition eauto.
+  Qed.
+End StepPreSync.
+
+Module Exec.
+
+  Inductive R {sync_R: rawdisk -> rawdisk -> Prop} : forall T, rawdisk -> hashmap -> prog T -> outcome T -> Prop :=
+  | XRet : forall T m hm (v: T),
+      R m hm (Ret v) (Finished m hm v)
+  | XStep : forall T m hm (p: prog T) m' m'' hm' v,
+      step m hm p m' hm' v ->
+      sync_R m' m'' ->
+      R m hm p (Finished m'' hm' v)
+  | XBindFinish : forall m hm T (p1: prog T) m' hm' (v: T)
+                    T' (p2: T -> prog T') out,
+      R m hm p1 (Finished m' hm' v) ->
+      R m' hm' (p2 v) out ->
+      R m hm (Bind p1 p2) out
+  | XBindFail : forall m hm T (p1: prog T)
+                  T' (p2: T -> prog T'),
+      R m hm p1 (Failed T) ->
+      R m hm (Bind p1 p2) (Failed T')
+  | XBindCrash : forall m hm T (p1: prog T) m' hm'
+                   T' (p2: T -> prog T'),
+      R m hm p1 (Crashed T m' hm') ->
+      R m hm (Bind p1 p2) (Crashed T' m' hm')
+  | XFail : forall m hm T (p: prog T),
+      fail_step m p ->
+      R m hm p (Failed T)
+  | XCrash : forall m hm T (p: prog T),
+      crash_step p ->
+      R m hm p (Crashed T m hm).
+
+  Arguments R sync_R {T} _ _ _ _.
+End Exec.
+
+Hint Constructors Exec.R.
+Hint Constructors exec.
+
+Theorem exec_is_exec_possible_sync : forall T (p: prog T) m hm out,
+    exec m hm p out <->
+    Exec.R possible_sync m hm p out.
+Proof.
+  split; induction 1; eauto.
+Qed.
+
+(* if out is ok, out' is at least as ok *)
+Definition outcome_obs_le T (out out': outcome T) : Prop :=
+  match out with
+  | Failed _ => out' = Failed T
+  | Finished d hm v => exists d', out' = Finished d' hm v /\
+                            possible_sync (AEQ:=addr_eq_dec) d d'
+  | Crashed _ d hm => exists d', out' = Crashed T d' hm /\
+                         possible_sync (AEQ:=addr_eq_dec) d d'
+  end.
+
+Definition outcome_obs_ge T (out' out: outcome T) : Prop :=
+  match out' with
+  | Failed _ => out = Failed T
+  | Finished d' hm v => exists d, out = Finished d hm v /\
+                             possible_sync (AEQ:=addr_eq_dec) d d'
+  | Crashed _ d' hm => exists d, out = Crashed T d hm /\
+                           possible_sync (AEQ:=addr_eq_dec) d d'
+  end.
+
+Theorem outcome_obs_ge_ok : forall T (out out': outcome T),
+    outcome_obs_le out out' <->
+    outcome_obs_ge out' out.
+Proof.
+  destruct out, out'; simpl; intuition idtac;
+    repeat deex;
+    match goal with
+    | [ H: @eq (outcome _) _ _ |- _ ] => inversion H; subst
+    end; eauto.
+Qed.
+
+Theorem outcome_obs_le_refl : forall T (out: outcome T),
+    outcome_obs_le out out.
+Proof.
+  destruct out; simpl; eauto.
+Qed.
+
+Theorem outcome_obs_le_trans : forall T (out out' out'': outcome T),
+    outcome_obs_le out out' ->
+    outcome_obs_le out' out'' ->
+    outcome_obs_le out out''.
+Proof.
+  destruct out, out'; intros; simpl in *; repeat deex; try congruence; eauto.
+  inversion H0; subst; eauto.
+  inversion H0; subst; eauto.
+Qed.
+
+Instance outcome_obs_le_preorder {T} : PreOrder (outcome_obs_le (T:=T)).
+Proof.
+  constructor; hnf; intros; eauto using outcome_obs_le_refl, outcome_obs_le_trans.
+Qed.
+
+Hint Resolve outcome_obs_le_refl outcome_obs_le_trans.
+
+Lemma possible_sync_in_domain : forall AT AEQ (d d': @mem AT AEQ _) a v vs',
+    possible_sync d d' ->
+    d' a = Some (v, vs') ->
+    exists vs, d a = Some (v, vs) /\
+          incl vs' vs.
+Proof.
+  unfold possible_sync; intros.
+  specialize (H a); intuition eauto; try congruence.
+  repeat deex.
+  assert (v = v0) by congruence; subst.
+  assert (l' = vs') by congruence; subst.
+  eauto.
+Qed.
+
+Hint Resolve ListUtils.incl_cons2.
+Hint Resolve incl_refl.
+Hint Resolve possible_sync_respects_sync_mem.
+
+Lemma step_sync_later : forall T (p: prog T) d d' d'' hm hm' v,
+    possible_sync d d' ->
+    step d' hm p d'' hm' v ->
+    exists d'2, step d hm p d'2 hm' v /\
+           possible_sync (AEQ:=addr_eq_dec) d'2 d''.
+Proof.
+  intros.
+  inversion H0; subst; repeat sigT_eq.
+  - (* Read *)
+    eapply possible_sync_in_domain in H8; eauto; deex.
+    eauto.
+  - eapply possible_sync_in_domain in H8; eauto; deex.
+    eexists; split.
+    constructor; eauto.
+    eapply possible_sync_respects_upd; eauto.
+  - eauto.
+  - destruct vs, vs'.
+    eapply possible_sync_in_domain in H8; eauto; deex.
+    eexists; split.
+    econstructor; eauto.
+    eapply possible_sync_respects_upd; eauto.
+  - eauto.
+Qed.
+
+Lemma possible_sync_not_in_domain : forall AT AEQ (d d': @mem AT AEQ _) a,
+    possible_sync d d' ->
+    d' a = None ->
+    d a = None.
+Proof.
+  unfold possible_sync; intros.
+  specialize (H a); intuition eauto;
+    repeat deex; congruence.
+Qed.
+
+Hint Resolve possible_sync_not_in_domain.
+Hint Constructors fail_step.
+
+Lemma fail_step_sync_later  : forall T (p: prog T) d d',
+    fail_step d' p ->
+    possible_sync d d' ->
+    fail_step d p.
+Proof.
+  inversion 1; intros; subst; repeat sigT_eq; eauto.
+Qed.
+
+Theorem exec_eq_sync_later : forall T (p: prog T) d d' hm out,
+    Exec.R eq d' hm p out ->
+    possible_sync d d' ->
+    exists out', Exec.R eq d hm p out' /\
+            outcome_obs_ge out out'.
+Proof.
+  intros.
+  generalize dependent d.
+  induction H; subst; intros; simpl.
+  - eexists; intuition eauto; simpl; eauto.
+  - eapply step_sync_later in H0; eauto; deex.
+    eexists; intuition eauto.
+  - specialize (IHR1 _ H1); deex.
+    simpl in *; deex.
+    specialize (IHR2 _ H5); deex.
+    eauto 10.
+  - specialize (IHR _ H0); deex.
+    simpl in *; subst.
+    eauto 10.
+  - specialize (IHR _ H0); deex.
+    simpl in *; deex.
+    eauto 10.
+  - eapply fail_step_sync_later in H; eauto.
+  - inversion H; subst; repeat sigT_eq; eauto 10.
+Qed.
+
+Theorem exec_sync_obs_irrelevant : forall T (p: prog T) d hm out,
+    Exec.R possible_sync d hm p out ->
+    exists out', Exec.R eq d hm p out' /\
+            outcome_obs_le out' out.
+Proof.
+  induction 1; intros; repeat deex; eauto.
+  - eexists; intuition eauto.
+    simpl.
+    eauto.
+  - destruct out'0; simpl in *; repeat deex; try congruence.
+    inversion H5; subst.
+    (* m ---> m0, m0 ~~> d', d' ---> out' <= out *)
+    eapply exec_eq_sync_later in H4; eauto; deex.
+    simpl in *; deex.
+    assert (possible_sync (AEQ:=addr_eq_dec) d d') by eauto.
+    eapply exec_eq_sync_later in H1; eauto; deex.
+    apply outcome_obs_ge_ok in H9.
+    eauto.
+  - destruct out'; simpl in *; repeat deex; try congruence.
+    eauto.
+  - destruct out'; simpl in *; repeat deex; try congruence.
+    inversion H2; subst.
+    eexists; intuition eauto.
+    simpl; eauto.
+Qed.
+
+Module ExecRecover.
+
+  Inductive R
+            {exec: forall T, rawdisk -> hashmap -> prog T -> outcome T -> Prop}
+            {possible_crash: rawdisk -> rawdisk -> Prop}
+            (TF TR: Type)
+  : rawdisk -> hashmap -> prog TF -> prog TR -> recover_outcome TF TR -> Prop :=
+  | XRFail : forall m hm p1 p2,
+      exec _ m hm p1 (Failed TF)
+      -> R m hm p1 p2 (RFailed TF TR)
+  | XRFinished : forall m hm p1 p2 m' hm' (v: TF),
+      exec _ m hm p1 (Finished m' hm' v)
+      -> R m hm p1 p2 (RFinished TR m' hm' v)
+  | XRCrashedFailed : forall m hm p1 p2 m' hm' m'r,
+      exec _ m hm p1 (Crashed TF m' hm')
+      -> possible_crash m' m'r
+      -> R (TF:=TR) m'r hm' p2 p2 (RFailed TR TR)
+      -> R m hm p1 p2 (RFailed TF TR)
+  | XRCrashedFinished : forall m hm p1 p2 m' hm' m'r m'' hm'' (v: TR),
+      exec _ m hm p1 (Crashed TF m' hm')
+      -> possible_crash m' m'r
+      -> R (TF:=TR) m'r hm' p2 p2 (RFinished TR m'' hm'' v)
+      -> R m hm p1 p2 (RRecovered TF m'' hm'' v)
+  | XRCrashedRecovered : forall m hm p1 p2 m' hm' m'r m'' hm'' (v: TR),
+      exec _ m hm p1 (Crashed TF m' hm')
+      -> possible_crash m' m'r
+      -> R (TF:=TR) m'r hm' p2 p2 (RRecovered TR m'' hm'' v)
+      -> R m hm p1 p2 (RRecovered TF m'' hm'' v).
+
+End ExecRecover.
+
+Arguments ExecRecover.R exec possible_crash {TF TR} _ _ _ _ _.
+
+Definition routcome_disk_R (R: rawdisk -> rawdisk -> Prop)
+           TF TR (out out': recover_outcome TF TR) :=
+  match out with
+  | RFinished _ d hm v => exists d', out' = RFinished _ d' hm v /\
+                               R d d'
+  | RRecovered _ d hm v => exists d', out' = RRecovered _ d' hm v /\
+                                R d d'
+  | RFailed _ _ => out' = RFailed _ _
+  end.
+
+Definition routcome_disk_R_conv (R: rawdisk -> rawdisk -> Prop)
+           TF TR (out' out: recover_outcome TF TR) :=
+  match out' with
+  | RFinished _ d hm v => exists d', out = RFinished _ d' hm v /\
+                               R d' d
+  | RRecovered _ d hm v => exists d', out = RRecovered _ d' hm v /\
+                                R d' d
+  | RFailed _ _ => out = RFailed _ _
+  end.
+
+Theorem routcome_disk_R_conv_ok : forall R TF TR (out out': recover_outcome TF TR),
+    routcome_disk_R R out out' <->
+    routcome_disk_R_conv R out' out.
+Proof.
+  split;
+    destruct out, out'; simpl; intros;
+      repeat deex;
+      match goal with
+      | [ H: @eq (recover_outcome _ _) _ _ |- _ ] =>
+        inversion H; subst
+      end; eauto.
+Qed.
+
+Hint Constructors ExecRecover.R exec_recover.
+
+Theorem exec_recover_is_R : forall TF TR d hm (p: prog TF) (r: prog TR) out,
+    exec_recover d hm p r out <->
+    ExecRecover.R exec possible_crash d hm p r out.
+Proof.
+  split; induction 1; eauto.
+Qed.
+
+Theorem exec_recover_without_sync : forall TF TR d hm (p: prog TF) (r: prog TR) out,
+    ExecRecover.R (@Exec.R possible_sync) possible_crash d hm p r out ->
+    exists out', ExecRecover.R (@Exec.R eq) possible_crash d hm p r out' /\
+            routcome_disk_R possible_sync out' out.
+Proof.
+  induction 1; simpl;
+    repeat match goal with
+           | [ H: Exec.R possible_sync _ _ _ _ |- _ ] =>
+             apply exec_sync_obs_irrelevant in H; simpl in H
+           | [ H: outcome_obs_le _ _ |- _ ] =>
+             apply outcome_obs_ge_ok in H; progress simpl in H
+           | [ H: routcome_disk_R _ _ _ |- _ ] =>
+             apply routcome_disk_R_conv_ok in H; progress simpl in H
+           | [ H: possible_sync ?m ?m',
+                  H': possible_crash ?m' ?m'' |- _ ] =>
+             lazymatch goal with
+             | [ H: possible_crash m m'' |- _ ] => fail
+             | _ => pose proof possible_crash_possible_sync_trans H H'
+             end
+           | _ => progress subst
+           | _ => deex
+           end;
+    try solve [ eexists; intuition eauto; simpl; eauto ].
+Qed.
+
+Module PhysicalSemantics.
+
+  (* we will now _re-interpret_ a valubuf as the following:
+
+     a |-> (v, vs) means v is the current value while the disk contains the
+     sequence of values vs, where the last value is on disk and the earlier
+     values are buffered. *)
+
+  (* partially flush each address by removing some old values and leaving a new
+  value on disk *)
+  Definition flush_disk (d d': rawdisk) :=
+    forall a,
+      match d a with
+      | None => d' a = None
+      | Some (v, vs) => exists n, d' a = Some (v, firstn n vs)
+      end.
+
+  Theorem flush_disk_refl : forall d, flush_disk d d.
+  Proof.
+    unfold flush_disk; intros.
+    destruct (d a) as [ [? ?] | ]; auto.
+    exists (length l).
+    rewrite firstn_all.
+    eauto.
+  Qed.
+
+  Theorem flush_disk_trans : forall d d' d'',
+      flush_disk d d' ->
+      flush_disk d' d'' ->
+      flush_disk d d''.
+  Proof.
+    unfold flush_disk; intros.
+    specialize (H a).
+    specialize (H0 a).
+    destruct (d a) as [ [? ?] | ];
+      destruct (d' a) as [ [? ?] | ];
+      repeat deex;
+      inv_opt;
+      try congruence.
+    rewrite firstn_firstn in H0.
+    eauto.
+  Qed.
+
+  Lemma firstn_incl : forall A (l: list A) n,
+      incl (firstn n l) l.
+  Proof.
+    unfold incl.
+    apply ListUtils.in_firstn_in.
+  Qed.
+
+  Hint Resolve firstn_incl.
+
+  Theorem flush_disk_is_sync : forall d d',
+      flush_disk d d' ->
+      possible_sync (AEQ:=addr_eq_dec) d d'.
+  Proof.
+    unfold flush_disk, possible_sync; intros.
+    specialize (H a).
+    destruct (d a); eauto.
+    right.
+    destruct p; deex; eauto 10.
+  Qed.
+
+  Hint Resolve flush_disk_is_sync.
+
+  (* with the new interpretation of valusets, the last value in (v, vs),
+  organized as v::vs, is the on-disk value *)
+  Fixpoint diskval (v: valu) (vs: list valu) :=
+    match vs with
+    | nil => v
+    | v'::vs' => diskval v' vs'
+    end.
+
+  (* discard buffers is actually a function  *)
+  Definition discard_buffers (d d': rawdisk) :=
+    forall a, match d a with
+         | None => d' a = None
+         | Some (v, vs) =>
+           d' a = Some (diskval v vs, nil)
+         end.
+
+  Lemma discard_buffers_f (d: rawdisk) : {d':rawdisk | discard_buffers d d'}.
+  Proof.
+    unfold discard_buffers.
+    exists (fun a =>
+         match d a with
+         | None => None
+         | Some (v, vs) =>
+           Some (diskval v vs, nil)
+         end).
+    intros.
+    destruct (d a); auto.
+    destruct p; auto.
+  Qed.
+
+  Remark discard_buffers_deterministic : forall d d' d'',
+      discard_buffers d d' ->
+      discard_buffers d d'' ->
+      d' = d''.
+  Proof.
+    unfold discard_buffers; intros.
+    extensionality a.
+    specialize (H a).
+    specialize (H0 a).
+    destruct (d a) as [ [? ?] | ]; congruence.
+  Qed.
+
+  Definition outcome_disk_R (R: rawdisk -> rawdisk -> Prop) T (out out':outcome T) :=
+    match out with
+    | Finished d hm v => exists d', out' = Finished d' hm v /\
+                              R d d'
+    | Crashed _ d hm => exists d', out' = Crashed _ d' hm /\
+                           R d d'
+    | Failed _ => out' = Failed _
+    end.
+
+  Definition pexec T d hm (p: prog T) out :=
+    exists out', Exec.R flush_disk d hm p out' /\
+          outcome_disk_R flush_disk out' out.
+  Definition pexec_recover := @ExecRecover.R pexec discard_buffers.
+
+  Hint Resolve flush_disk_refl flush_disk_trans.
+  Hint Resolve flush_disk_is_sync.
+
+  Lemma flush_disk_in_domain : forall d d' a v vs,
+      d a = Some (v, vs)  ->
+      flush_disk d d' ->
+      exists n, d' a = Some (v, firstn n vs).
+  Proof.
+    unfold flush_disk; intros.
+    specialize (H0 a).
+    rewrite H in H0; eauto.
+  Qed.
+
+  Theorem outcome_obs_le_to_R : forall T (out out': outcome T),
+      outcome_obs_le out out' <->
+      outcome_disk_R possible_sync out out'.
+  Proof.
+    unfold outcome_obs_le, outcome_disk_R; split; intros;
+      destruct out; eauto.
+  Qed.
+
+  (* We want to prove that using the non-deterministic crash (our actual
+  semantics) is sufficient for safety under the real, deterministic crash +
+  non-deterministic flush (the above semantics). This is guaranteed by proving
+  if exec_real -> (exists out, exec_fake to out) -> exec_real's out is
+  similar *)
+
+  (* similarity is vague - want all the values to match for correctness, and to
+  get proof to go through need the write buffers in the real execution to be
+  sensible *)
+
+  Lemma exec_flush_to_exec : forall T (p: prog T) d hm out,
+      Exec.R flush_disk d hm p out ->
+      exec d hm p out.
+  Proof.
+    induction 1; simpl; intros;
+      intuition (repeat deex; eauto 10).
+  Qed.
+
+  Corollary pexec_to_exec : forall T (p: prog T) d hm out,
+      pexec d hm p out ->
+      exists out', exec d hm p out' /\
+              outcome_disk_R flush_disk out' out.
+  Proof.
+    unfold pexec; intros; deex.
+    eauto using exec_flush_to_exec.
+  Qed.
+
+  Definition outcome_disk_R_conv (R: rawdisk -> rawdisk -> Prop)
+             T (out' out: outcome T) :=
+   match out' with
+   | Finished m hm v => exists m', out = Finished m' hm v /\
+                               R m' m
+   | Crashed _ m hm => exists m', out = Crashed _ m' hm /\
+                            R m' m
+   | Failed _ => out = Failed  _
+   end.
+
+  Theorem outcome_disk_R_conv_ok : forall R T (out out': outcome T),
+      outcome_disk_R R out out' <->
+      outcome_disk_R_conv R out' out.
+  Proof.
+    unfold outcome_disk_R, outcome_disk_R_conv; split; intros;
+      destruct out, out'; repeat deex; try congruence.
+    inversion H0; eauto.
+    inversion H0; eauto.
+    inversion H0; eauto.
+    inversion H0; eauto.
+  Qed.
+
+
+  Lemma diskval_firstn_in_list : forall l n v,
+      In (diskval v (firstn n l)) (v::l).
+  Proof.
+    induction l; simpl; intros.
+    rewrite firstn_nil; eauto.
+    destruct n; simpl; eauto.
+    destruct (IHl n a); simpl; eauto.
+  Qed.
+
+  Theorem discard_flush_is_crash : forall d d' d'',
+      flush_disk d d' ->
+      discard_buffers d' d'' ->
+      possible_crash d d''.
+  Proof.
+    unfold flush_disk, discard_buffers, possible_crash; intros.
+    specialize (H a).
+    specialize (H0 a).
+    destruct (d a) as [ [? ?] | ];
+      destruct (d' a) as [ [? ?] | ];
+      repeat deex;
+      inv_opt;
+      try congruence;
+      eauto.
+    right.
+    repeat eexists; eauto.
+    apply diskval_firstn_in_list.
+  Qed.
+
+  Hint Constructors exec_recover.
+
+  Theorem pexec_recover_to_exec_recover : forall TF TR (p: prog TF) (r: prog TR) d hm out,
+      pexec_recover d hm p r out ->
+      exists out', exec_recover d hm p r out' /\
+              routcome_disk_R possible_sync out' out.
+  Proof.
+    induction 1; simpl;
+      repeat match goal with
+             | [ H: pexec _ _ _ _ |- _ ] =>
+               apply pexec_to_exec in H; simpl in H; deex
+             | [ H: outcome_disk_R _ _ _ |- _ ] =>
+               apply outcome_disk_R_conv_ok in H; progress simpl in H
+             | [ H: routcome_disk_R _ _ _ |- _ ] =>
+               apply routcome_disk_R_conv_ok in H; progress simpl in H
+             | [ H: flush_disk ?d ?d',
+                    H' : discard_buffers ?d' ?d'' |- _ ] =>
+               lazymatch goal with
+               | [ H: possible_crash d d'' |- _ ] => fail
+               | _ => pose proof (discard_flush_is_crash H H')
+               end
+             | _ => progress subst
+             | _ => deex
+             end;
+      try solve [ eexists; intuition eauto; simpl; eauto ].
+  Qed.
+
+End PhysicalSemantics.
